code/ecdsa/Hacl.Impl.EC.PointAddMixed.fst
@@ -1,5 +1,4 @@
 module Hacl.Impl.EC.PointAddMixed
-
 open FStar.HyperStack.All
 open FStar.HyperStack
 module ST = FStar.HyperStack.ST
@@ -18,93 +17,111 @@ open FStar.Tactics.Canon
 
 open FStar.Math.Lemmas
 open Hacl.Impl.EC.Masking
-open Hacl.Spec.EC.Definition
 
-
-friend Hacl.Impl.EC.PointAdd
 open Hacl.Spec.MontgomeryMultiplication
 open FStar.Mul
 
-open Hacl.Impl.P.PointAddMixed.Aux
-
-#set-options "--z3rlimit 300 --fuel 0 --ifuel 0"
+open Hacl.Impl.P.PointAdd.Aux
 
 
-(* during the precomputation of points we want to express a point at infinity. We present is as a point such that both coordinates are equal to zero *)
+#set-options "--z3rlimit 300 --ifuel 0 --fuel 0"  
+
+
 
 inline_for_extraction noextract 
-val pointAffineIsNotZero: #c: curve ->
-  #buf_type: buftype -> p: lbuffer_t buf_type uint64 (size 2 *! getCoordinateLenU64 c) -> Stack uint64
+val pointAffineIsNotZero: #c: curve -> #buf_type : buftype ->  p: lbuffer_t buf_type uint64 (size 8) -> Stack uint64
   (requires fun h -> live h p)
-  (ensures fun h0 r h1 -> modifies0 h0 h1 /\ (
-    let len = getCoordinateLenU64 c in 
-    let x = lseq_as_nat (as_seq h0 (gsub p (size 0) len)) in 
-    let y = lseq_as_nat (as_seq h0 (gsub p len len)) in 
-    if isPointAtInfinityAffine (x, y) then uint_v r = pow2 64 - 1 else uint_v r == 0))
-
+  (ensures fun h0 r h1 -> modifies0 h0 h1)
 
 let pointAffineIsNotZero #c p = 
-  let h0 = ST.get() in 
-  
-  let len = getCoordinateLenU64 c in 
-  let x = sub p (size 0) len in 
-  let y = sub p len len in 
+  let x = sub p (size 0) (size 4) in 
+  let y = sub p (size 4) (size 4) in 
 
   let xZero = isZero_uint64_CT #c x in 
   let yZero = isZero_uint64_CT #c y in 
+
+(*   let xZero = eq_felem_0_u64 (global_to_comparable x) in 
+  let yZero = eq_felem_0_u64 (global_to_comparable y) in  *)
 
   logand_lemma xZero yZero;
   logand xZero yZero
 
 
-val copy_point_conditional: #c: curve -> result: point c -> p: point c -> mask: point c ->
+inline_for_extraction noextract
+val copy_point_conditional: #c: curve -> x3_out: felem c -> y3_out: felem c -> z3_out: felem c -> p: point c -> mask: point c ->
   Stack unit
-  (requires fun h -> point_eval c h mask /\ point_eval c h p /\ point_eval c h result /\
-    live h result /\ live h p /\ live h mask /\ 
-    LowStar.Monotonic.Buffer.all_disjoint [loc result; loc p; loc mask])
-  (ensures fun h0 _ h1 -> modifies (loc result) h0 h1 /\ point_eval c h1 result /\ (
+  (requires fun h -> point_eval c h mask /\ point_eval c h p /\
+    live h x3_out /\ live h y3_out /\ live h z3_out /\ live h p /\ live h mask /\ 
+    LowStar.Monotonic.Buffer.all_disjoint [loc x3_out; loc y3_out; loc z3_out; loc p; loc mask])
+  (ensures fun h0 _ h1 -> modifies (loc x3_out |+| loc y3_out |+| loc z3_out) h0 h1 /\ (
     let mask = point_z_as_nat c h0 mask in 
+    let x, y, z = point_x_as_nat c h0 p, point_y_as_nat c h0 p, point_z_as_nat c h0 p in
     if mask = 0 then
-      point_x_as_nat c h1 result == point_x_as_nat c h0 p /\
-      point_y_as_nat c h1 result == point_y_as_nat c h0 p /\ 
-      point_z_as_nat c h1 result == point_z_as_nat c h0 p
+      as_nat c h1 x3_out == x /\
+      as_nat c h1 y3_out == y /\ 
+      as_nat c h1 z3_out == z
     else 
-      point_x_as_nat c h1 result == point_x_as_nat c h0 result /\ 
-      point_y_as_nat c h1 result == point_y_as_nat c h0 result /\ 
-      point_z_as_nat c h1 result == point_z_as_nat c h0 result))
+      as_nat c h1 x3_out == as_nat c h0 x3_out /\ 
+      as_nat c h1 y3_out == as_nat c h0 y3_out /\ 
+      as_nat c h1 z3_out == as_nat c h0 z3_out))
 
-let copy_point_conditional #c result p mask = 
-  let len = getCoordinateLenU64 c in
+
+let copy_point_conditional #c x3_out y3_out z3_out p maskPoint = 
+  [@inline_let]
+  let len = getCoordinateLenU64 c in 
   
-  let mask = isZero_uint64_CT #c (sub mask (size 2 *! len) len) in 
-
-  let outX = sub result (size 0) len in 
-  let outY = sub result len len in 
-  let outZ = sub result (size 2 *! len) len in 
-
-  let pX = sub p (size 0) len in 
-  let pY = sub p len len in 
-  let pZ = sub p (size 2 *! len) len in 
-
-  copy_conditional #c outX pX mask;
-  copy_conditional #c outY pY mask;
-  copy_conditional #c outZ pZ mask
+  let z = sub maskPoint (size 2 *! len) len in 
+  let mask = isZero_uint64_CT #c z in 
   
+  let p_x = sub p (size 0) len in 
+  let p_y = sub p len len in 
+  let p_z = sub p (size 2 *! len) len in 
+
+  copy_conditional x3_out p_x mask;
+  copy_conditional y3_out p_y mask;
+  copy_conditional z3_out p_z mask
+
+
+inline_for_extraction noextract
+val copy_point_conditional1: #c: curve -> x3_out: felem c -> y3_out: felem c -> z3_out: felem c ->  p: point c -> mask: felem c ->
+  Stack unit
+  (requires fun h -> True)
+  (ensures fun h0 _ h1 -> True)
+
+
+let copy_point_conditional1 #c x3_out y3_out z3_out p mask = 
+  [@inline_let]
+  let len = getCoordinateLenU64 c in 
+
+(*   let x3_out = sub result (size 0) len in 
+  let y3_out = sub result len len in 
+  let z3_out = sub result (2ul *! len) len in
+ *)
+  let p_x = sub p (size 0) len in 
+  let p_y = sub p len len in 
+  let p_z = sub p (size 2 *! len) len in 
+
+  copy_conditional x3_out p_x mask;
+  copy_conditional y3_out p_y mask;
+  copy_conditional z3_out p_z mask
+
+
+
 
 inline_for_extraction noextract 
 val _move_from_jacobian_coordinates: #c: curve -> u1: felem c -> u2: felem c -> 
-  s1: felem c -> s2: felem c -> p: point c -> q: pointAffine c -> 
+  s1: felem c -> s2: felem c -> p: point c -> q: point c -> 
   tempBuffer4: lbuffer uint64 (size 4 *! getCoordinateLenU64 c) -> 
   Stack unit (requires fun h ->  
     live h u1 /\ live h u2 /\ live h s1 /\ live h s2 /\ live h tempBuffer4 /\ live h p /\ 
-    live h q /\ point_eval c h p /\  point_aff_eval c h q /\
+    live h q /\ point_eval c h p /\ point_eval c h q /\
     LowStar.Monotonic.Buffer.all_disjoint [loc tempBuffer4; loc p; loc q; loc u1; loc u2; loc s1; loc s2])
   (ensures fun h0 _ h1 ->  
-    modifies (loc u1 |+| loc u2 |+| loc s1 |+| loc s2 |+| loc tempBuffer4) h0 h1 (*/\
+    modifies (loc u1 |+| loc u2 |+| loc s1 |+| loc s2 |+| loc tempBuffer4) h0 h1 /\
     u1Invariant #c h0 h1 u1 p q /\
     u2Invariant #c h0 h1 u2 p q /\ 
     s1Invariant #c h0 h1 s1 p q /\
-    s2Invariant #c h0 h1 s2 p q *))
+    s2Invariant #c h0 h1 s2 p q)
 
 
 let _move_from_jacobian_coordinates #c u1 u2 s1 s2 p q tempBuffer = 
@@ -119,6 +136,7 @@ let _move_from_jacobian_coordinates #c u1 u2 s1 s2 p q tempBuffer =
 
   let qX = sub q (size 0) len in 
   let qY = sub q len len in 
+  (* let qZ = sub q (size 2 *! len) len in   *)
 
   let z2Square = sub tempBuffer (size 0) len in 
   let z1Square = sub tempBuffer len len in 
@@ -127,15 +145,15 @@ let _move_from_jacobian_coordinates #c u1 u2 s1 s2 p q tempBuffer =
 
   let h0 = ST.get() in 
 
-   upd z2Square (size 0) (u64 0x000000300000000);
-   upd z2Square (size 1) (u64 0x00000001FFFFFFFE);
-   upd z2Square (size 2) (u64 0xFFFFFFFD00000002);
-   upd z2Square (size 3) (u64 0xFFFFFFFE00000003);
+  upd z2Square (size 0) (u64 0x000000300000000);
+  upd z2Square (size 1) (u64 0x00000001FFFFFFFE);
+  upd z2Square (size 2) (u64 0xFFFFFFFD00000002);
+  upd z2Square (size 3) (u64 0xFFFFFFFE00000003);
 
-    upd z2Cube (size 0) (u64 0x0000000CFFFFFFF7);
-    upd z2Cube (size 1) (u64 0xFFFFFFF800000007); 
-    upd z2Cube (size 2) (u64 0xFFFFFFFB0000000F);
-    upd z2Cube (size 3) (u64 0x00000005FFFFFFFF);
+  upd z2Cube (size 0) (u64 0x0000000CFFFFFFF7);
+  upd z2Cube (size 1) (u64 0xFFFFFFF800000007); 
+  upd z2Cube (size 2) (u64 0xFFFFFFFB0000000F);
+  upd z2Cube (size 3) (u64 0x00000005FFFFFFFF);
 
 
   (* montgomery_square_buffer_dh #c qZ z2Square;  *)
@@ -150,9 +168,9 @@ let _move_from_jacobian_coordinates #c u1 u2 s1 s2 p q tempBuffer =
   montgomery_multiplication_buffer_dh #c z2Cube pY s1;
   montgomery_multiplication_buffer_dh #c z1Cube qY s2;
 
-  let prime = getPrime c in 
+  let prime = getPrime c in ()
   
-  let fromDomain = fromDomain #c in 
+(*   let fromDomain = fromDomain #c in 
   let toDomain = toDomain #c in   
   let as_nat = as_nat c in 
 
@@ -163,7 +181,7 @@ let _move_from_jacobian_coordinates #c u1 u2 s1 s2 p q tempBuffer =
   let qyD = fromDomain (as_nat h0 qY) in 
 
   let pzD = fromDomain (as_nat h0 pZ) in 
-  let qzD = fromDomain 1 in 
+  let qzD = fromDomain (as_nat h0 qZ) in 
 
 
   calc (==)
@@ -199,10 +217,10 @@ let _move_from_jacobian_coordinates #c u1 u2 s1 s2 p q tempBuffer =
     (==) {lemma_mod_mul_distr_l (pzD * pzD * pzD) qyD prime}
     toDomain(pzD * pzD * pzD * qyD % prime);
   }
-
+ *)
 
 inline_for_extraction noextract 
-val move_from_jacobian_coordinates_mixed: #c: curve -> p: point c -> q: pointAffine c -> 
+val move_from_jacobian_coordinates: #c: curve -> p: point c -> q: point c -> 
   t12: lbuffer uint64 (size 12 *! getCoordinateLenU64 c) -> 
   Stack unit (requires fun h -> 
     live h t12 /\ live h p /\ live h q /\
@@ -217,7 +235,7 @@ val move_from_jacobian_coordinates_mixed: #c: curve -> p: point c -> q: pointAff
     s2Invariant #c h0 h1 s2 p q))
 
 
-let move_from_jacobian_coordinates_mixed #c p q t12 = 
+let move_from_jacobian_coordinates #c p q t12 = 
   [@inline_let]
   let len = getCoordinateLenU64 c in   
   
@@ -231,87 +249,248 @@ let move_from_jacobian_coordinates_mixed #c p q t12 =
   _move_from_jacobian_coordinates #c u1 u2 s1 s2 p q t4
 
 
+inline_for_extraction noextract
+val compute_common_params_point_add: #c: curve 
+  -> t12: lbuffer uint64 (size 12 *! getCoordinateLenU64 c) -> 
+  Stack unit 
+  (requires fun h0 -> live h0 t12 /\ (
+    let u1, u2, s1, s2, _, _, _, _ = getU1HCube t12 in  
+    felem_eval c h0 u1 /\ felem_eval c h0 u2 /\ felem_eval c h0 s1 /\ felem_eval c h0 s2))
+  (ensures fun h0 _ h1 -> 
+    let  u1, u2, s1, s2, h, r, uh, hCube = getU1HCube t12 in 
+    modifies (loc t12) h0 h1 /\
+    as_nat c h0 u1 == as_nat c h1 u1 /\
+    as_nat c h0 u2 == as_nat c h1 u2 /\
+    as_nat c h0 s1 == as_nat c h1 s1 /\
+    as_nat c h0 s2 == as_nat c h1 s2 /\
+    
+    hInvariant #c h1 h u1 u2 /\
+    rInvariant #c h1 r s1 s2 /\
+    uhInvariant #c h1 uh h u1 /\
+    hCubeInvariant #c h1 hCube h)
 
-inline_for_extraction noextract 
-val computeZ3_point_add_mixed: #c: curve -> z3: felem  c -> z1: felem c -> 
-  h: felem c -> tempBuffer: felem c -> 
-  Stack unit
-  (requires fun h0 -> 
-    live h0 z3 /\ live h0 z1 /\ live h0 h /\  live h0 tempBuffer /\
-    disjoint z3 z1 /\ disjoint z1 tempBuffer /\ disjoint tempBuffer h /\ disjoint h z3 /\
-    felem_eval c h0 z1 /\ felem_eval c h0 h)
-  (ensures fun h0 _ h1 -> modifies (loc z3 |+| loc tempBuffer) h0 h1 /\ (
-    let z1D = fromDomain_ #c #DH (as_nat c h0 z1) in 
-    let hD = fromDomain_ #c #DH (as_nat c h0 h) in 
-    as_nat c h1 z3 == toDomain_ #c #DH (z1D * hD % getPrime c)))  
 
+let compute_common_params_point_add #c t12 =
+  [@inline_let]
+  let len = getCoordinateLenU64 c in
+  lemma_ICuttable_common #c; 
 
-let computeZ3_point_add_mixed #c z3 z1 h tempBuffer =    
-  let len = getCoordinateLenU64 c in 
-  let h0 = ST.get() in 
-  let z1z2 = sub tempBuffer (size 0) len in
-  montgomery_multiplication_buffer_by_one_dh z1 z1z2;
-    let h1 = ST.get() in 
-  montgomery_multiplication_buffer_dh z1z2 h z3;
-    let h2 = ST.get() in 
+  let temp = sub t12 (size 0) len in 
 
-  let z1D = fromDomain_ #c #DH (as_nat c h0 z1) in 
-  let hD = fromDomain_ #c #DH (as_nat c h0 h) in 
-  assert(as_nat c h1 z1z2 = z1D);
-  assert(as_nat c h2 z3 = toDomain_ #c #DH (fromDomain_ #c #DH z1D * hD % getPrime c));
-  
-  admit()
+  let u1 = sub t12 (size 4 *! len) len in 
+  let u2 = sub t12 (size 5 *! len) len in 
+  let s1 = sub t12 (size 6 *! len) len in 
+  let s2 = sub t12 (size 7 *! len) len in
+
+  let h = sub t12 (size 8 *! len) len in 
+  let r = sub t12 (size 9 *! len) len in 
+  let uh = sub t12 (size 10 *! len) len in
+  let hCube = sub t12 (size 11 *! len) len in 
+
+  felem_sub #c u2 u1 h; 
+  felem_sub #c s2 s1 r;    
+  montgomery_square_buffer_dh #c h temp;
+    let h1 = ST.get() in   
+  montgomery_multiplication_buffer_dh #c temp u1 uh;
+  montgomery_multiplication_buffer_dh #c temp h hCube;
+
+  let prime = getPrime c in 
+  lemma_mod_mul_distr_l (fromDomain #c (as_nat c h1 h) * fromDomain #c (as_nat c h1 h)) (fromDomain #c (as_nat c h1 u1)) prime;
+  lemma_mod_mul_distr_l (fromDomain #c (as_nat c h1 h) * fromDomain #c (as_nat c h1 h)) (fromDomain #c (as_nat c h1 h)) prime
 
 
 inline_for_extraction noextract
-val cmovznz_one_mm: #c: curve -> out: felem c -> mask: uint64 -> tempBuffer: felem c -> Stack unit
-  (requires fun h -> live h out /\ live h tempBuffer /\ disjoint out tempBuffer /\
-    (uint_v mask == 0 \/ uint_v mask = pow2 64 - 1))
-  (ensures fun h0 _ h1 -> modifies (loc out |+| loc tempBuffer) h0 h1 /\ (
-    if v mask = 0 then 
-      as_nat c h1 out == as_nat c h0 out 
-    else 
-      as_nat c h1 out == 1))
+val computex3_point_add: #c : curve -> hCube: felem c -> uh: felem c -> 
+  r: felem c -> t5: lbuffer uint64 (size 5 *! getCoordinateLenU64 c) ->  
+  Stack unit 
+  (requires fun h0 -> 
+    live h0 hCube /\ live h0 uh /\ live h0 r /\ live h0 t5 /\
+    disjoint hCube t5 /\ disjoint uh t5 /\ disjoint r t5 /\
+    felem_eval c h0 hCube /\ felem_eval c h0 uh /\ felem_eval c h0 r)
+  (ensures fun h0 _ h1 -> modifies (loc t5) h0 h1 /\ (
+    let x3 = gsub t5 (size 0) (getCoordinateLenU64 c) in
+    x3Invariant #c h0 h1 x3 r hCube uh))
 
-let cmovznz_one_mm #c out mask tempBuffer = 
-  uploadOneImpl tempBuffer;
-  copy_conditional out tempBuffer mask
+let computex3_point_add #c hCube uh r t4 = 
+    let h0 = ST.get() in
+  [@inline_let]
+  let len = getCoordinateLenU64 c in 
+  
+  let x3 = sub t4 (size 0) len in 
+  let rSquare = sub t4 len len in 
+  let rH = sub t4 (size 2 *! len) len in 
+  let twoUh = sub t4 (size 3 *! len) len in 
+  
+  montgomery_square_buffer_dh r rSquare; 
+  felem_sub rSquare hCube rH;
+  multByTwo uh twoUh;
+  felem_sub #c rH twoUh x3; 
+
+  let prime = getPrime c in 
+  let r = as_nat c h0 r in 
+
+  let as_nat = as_nat c in 
+  let toDomain = toDomain #c in 
+  let fromDomain = fromDomain #c in 
+  
+  calc (==)
+  {
+    toDomain (((((fromDomain r * fromDomain r  % prime) - fromDomain (as_nat h0 hCube)) % prime) - (2 * fromDomain (as_nat h0 uh) % prime)) % prime);
+    (==) {lemma_mod_add_distr (- fromDomain (as_nat h0 hCube)) (fromDomain r * fromDomain r) prime}
+    toDomain (((fromDomain r * fromDomain r - fromDomain (as_nat h0 hCube)) % prime - (2 * fromDomain (as_nat h0 uh) % prime)) % prime);
+    (==) {lemma_mod_sub_distr ((fromDomain r * fromDomain r - fromDomain (as_nat h0 hCube)) % prime) (2 * fromDomain (as_nat h0 uh)) prime}
+    toDomain (((fromDomain r * fromDomain r - fromDomain (as_nat h0 hCube)) % prime - (2 * fromDomain (as_nat h0 uh))) % prime);
+    (==) {lemma_mod_add_distr (- (2 * fromDomain (as_nat h0 uh))) ((fromDomain r * fromDomain r - fromDomain (as_nat h0 hCube))) prime}
+    toDomain ((fromDomain r * fromDomain r - fromDomain (as_nat h0 hCube) - (2 * fromDomain (as_nat h0 uh))) % prime);
+    (==) {_ by (canon())}
+    toDomain ((fromDomain r * fromDomain r - fromDomain (as_nat h0 hCube) - 2 * fromDomain (as_nat h0 uh)) % prime);
+  }
+
+
+inline_for_extraction noextract
+val computeY3_point_add: #c: curve -> s1: felem c -> hCube: felem c -> uh: felem c -> r: felem c 
+  -> t5: lbuffer uint64 (size 5 *! getCoordinateLenU64 c) -> 
+  Stack unit 
+  (requires fun h -> 
+    let x3_out = gsub t5 (size 0) (getCoordinateLenU64 c) in 
+    live h s1 /\ live h hCube /\ live h uh /\ live h r /\ live h t5 /\
+    disjoint uh t5 /\ disjoint r t5 /\ disjoint s1 t5 /\ disjoint hCube t5 /\ 
+    eq_or_disjoint s1 hCube /\ 
+    felem_eval c h s1 /\ felem_eval c h hCube /\ felem_eval c h uh /\ felem_eval c h x3_out /\ felem_eval c h r)
+  (ensures fun h0 _ h1 -> 
+    let len = getCoordinateLenU64 c in 
+    let x3_out = gsub t5 (size 0) len in 
+    let y3_out = gsub t5 len len in 
+    modifies (loc t5) h0 h1 /\
+    as_nat c h0 x3_out == as_nat c h1 x3_out /\
+    y3Invariant #c h0 h1 y3_out s1 hCube uh x3_out r)
+
+let computeY3_point_add #c s1 hCube uh r tempBuffer5 = 
+  let x3 = sub tempBuffer5 (size 0) (getCoordinateLenU64 c) in 
+  let y3 = sub tempBuffer5 (getCoordinateLenU64 c) (getCoordinateLenU64 c) in 
+
+  let h0 = ST.get() in
+
+  [@inline_let]
+  let len = getCoordinateLenU64 c in 
+  
+  let s1hCube = sub tempBuffer5 (size 2 *! getCoordinateLenU64 c) len in 
+  let u1hx3 = sub tempBuffer5 (size 3 *! getCoordinateLenU64 c) len in 
+  let ru1hx3 = sub tempBuffer5 (size 4 *! getCoordinateLenU64 c) len in 
+  
+  montgomery_multiplication_buffer_dh s1 hCube s1hCube;
+  felem_sub uh x3 u1hx3; 
+  montgomery_multiplication_buffer_dh u1hx3 r ru1hx3; 
+  felem_sub #c ru1hx3 s1hCube y3;
+
+  let h3 = ST.get() in 
+
+  let prime = getPrime c in
+
+  let s1D = fromDomain #c (as_nat c h0 s1) in 
+  let hCubeD = fromDomain #c (as_nat c h0 hCube) in 
+  let uhD = fromDomain #c (as_nat c h0 uh) in 
+  let x3D = fromDomain #c (as_nat c h0 x3) in 
+  let rD = fromDomain #c (as_nat c h0 r) in 
+
+  calc (==)
+  {
+    toDomain #c (((uhD - x3D) % prime * rD % prime  - (s1D * hCubeD % prime)) % getPrime c);
+    (==) {lemma_mod_mul_distr_l (uhD - x3D) rD prime}
+    toDomain #c (((uhD - x3D) * rD % prime  - (s1D * hCubeD % prime)) % getPrime c);
+    (==) {_ by (canon())}
+    toDomain #c (((uhD - x3D) * rD % prime  - s1D * hCubeD % prime) % getPrime c);
+    (==) {lemma_mod_sub_distr ((uhD - x3D) * rD % prime) (s1D * hCubeD) prime}
+    toDomain #c (((uhD - x3D) * rD % prime - s1D * hCubeD) % getPrime c);
+    (==) {lemma_mod_add_distr (-s1D * hCubeD) ((uhD - x3D) * rD) prime}
+    toDomain #c (((uhD - x3D) * rD - s1D * hCubeD) % getPrime c);
+  }
+
 
 
 inline_for_extraction noextract 
-val copy_point_conditional_affine_to_result: #c: curve -> #buf_type : buftype -> out: point c
-  -> q: lbuffer_t buf_type uint64 (size 8)
-  -> maskPoint: point c
-  -> tempBuffer: felem c 
-  -> Stack unit 
-  (requires fun h -> live h out /\ live h q /\ live h maskPoint /\ disjoint q out /\ eq_or_disjoint out maskPoint)
-  (ensures fun h0 _ h1 -> modifies (loc out) h0 h1)
+val computeZ3_point_add: #c: curve -> p: point c -> q: point c ->
+  h: felem c -> t5: lbuffer uint64 (size 5 *! getCoordinateLenU64 c) -> 
+  Stack unit 
+  (requires fun h0 -> 
+    live h0 t5 /\ live h0 p /\ live h0 q /\ live h0 h /\ 
+    disjoint t5 p /\ disjoint t5 h /\ disjoint t5 q /\ eq_or_disjoint p q /\
+    point_eval c h0 p /\ point_eval c h0 q /\ felem_eval c h0 h)
+  (ensures fun h0 _ h1 -> modifies (loc t5) h0 h1 /\ (
+    let len = getCoordinateLenU64 c in 
+    let z1, z2 = getZ p, getZ q in 
+    let x3, y3, z3 = getXYZ #c t5 in 
+    as_nat c h0 x3 == as_nat c h1 x3 /\
+    as_nat c h0 y3 == as_nat c h1 y3 /\
+    z3Invariant #c h0 h1 z3 z1 z2 h))
+
+let computeZ3_point_add #c p q h t5 = 
+    let h0 = ST.get() in 
+  [@inline_let]
+  let len = getCoordinateLenU64 c in 
+
+  let z1 = sub p (size 2 *! len) len in 
+  (* let z2 = sub q (size 2 *! len) len in  *)
+  let z3 = sub t5 (size 2 *! len) len in 
+  
+  let z1z2 = sub t5 (size 3 *! len) len in 
+
+  montgomery_multiplication_buffer_by_one_dh #c z1 z1z2;
+  montgomery_multiplication_buffer_dh #c z1z2 h z3 
+
+(* 
+  calc (==)
+  {
+    toDomain #c ((fromDomain #c (as_nat c h0 z1) * fromDomain #c (as_nat c h0 z2) % getPrime c) * fromDomain #c (as_nat c h0 h) % getPrime c);
+    (==) {lemma_mod_mul_distr_l (fromDomain #c (as_nat c h0 z1) * fromDomain #c (as_nat c h0 z2)) (fromDomain #c (as_nat c h0 h)) (getPrime c)}
+    toDomain #c (fromDomain #c (as_nat c h0 z1) * fromDomain #c (as_nat c h0 z2) * fromDomain #c (as_nat c h0 h) % getPrime c);}
+
+ *)
+
+inline_for_extraction noextract
+val copy_result_point_add: #c: curve 
+  -> t5: lbuffer uint64 (size 5 *! (getCoordinateLenU64 c)) 
+  -> p: point c -> q: point c -> result: point c ->
+  Stack unit 
+  (requires fun h -> live h t5 /\ live h p /\ live h q /\ live h result /\
+    eq_or_disjoint p result /\ disjoint t5 result /\ 
+    point_eval c h q /\ point_eval c h p /\
+    LowStar.Monotonic.Buffer.all_disjoint [loc t5; loc p; loc q])
+  (ensures fun h0 _ h1 -> 
+    let x3_out, y3_out, z3_out = getXYZ #c t5 in 
+    modifies (loc t5 |+| loc result) h0 h1 /\ point_eval c h1 result /\ (
+    if point_z_as_nat c h0 q = 0 then 
+      point_x_as_nat c h1 result == point_x_as_nat c h0 p /\
+      point_y_as_nat c h1 result == point_y_as_nat c h0 p /\ 
+      point_z_as_nat c h1 result == point_z_as_nat c h0 p
+    else if point_z_as_nat c h0 p = 0 then 
+      point_x_as_nat c h1 result == point_x_as_nat c h0 q /\
+      point_y_as_nat c h1 result == point_y_as_nat c h0 q /\ 
+      point_z_as_nat c h1 result == point_z_as_nat c h0 q
+    else 
+      point_x_as_nat c h1 result == as_nat c h0 x3_out /\ 
+      point_y_as_nat c h1 result == as_nat c h0 y3_out /\ 
+      point_z_as_nat c h1 result == as_nat c h0 z3_out))
 
 
-let copy_point_conditional_affine_to_result #c out q maskPoint tempBuffer = 
+let copy_result_point_add #c t5 p q result = 
   let h0 = ST.get() in 
-  
-  let pZ = sub maskPoint (size 8) (size 4) in 
-  let mask = isZero_uint64_CT #c pZ in
+  [@inline_let]
+  let len = getCoordinateLenU64 c in 
 
-  let xOut = sub out (size 0) (size 4) in 
-  let yOut = sub out (size 4) (size 4) in 
-  let zOut = sub out (size 8) (size 4) in 
-  
-  let qX = sub q (size 0) (size 4) in 
-  let qY = sub q (size 4) (size 4) in 
+  let x3_out = sub t5 (size 0) len in 
+  let y3_out = sub t5 len len in 
+  let z3_out = sub t5 (size 2 *! len) len in 
+
+  copy_point_conditional x3_out y3_out z3_out q p;
+  let mask = pointAffineIsNotZero #c q in 
+  copy_point_conditional1 x3_out y3_out z3_out p mask;
 
 
-   let qX = const_to_lbuffer qX in 
-   let qY = const_to_lbuffer qY in 
+  (* copy_point_conditional x3_out y3_out z3_out p q; *)
+  concat3 len x3_out len y3_out len z3_out result;
+  admit()
 
-  copy_conditional #c xOut qX mask;
-  copy_conditional #c yOut qY mask;
-  cmovznz_one_mm #c zOut mask tempBuffer;
-  
-(*
-  lemma_multiplication_not_mod_prime (as_nat h0 pZ); *)
-  lemmaFromDomain #c #DH (as_nat c h0 pZ)
 
 
 inline_for_extraction noextract
@@ -360,17 +539,20 @@ val computeXYZ: #c: curve -> result: point c
 let computeXYZ #c result p q u1 u2 s1 s2 r h uh hCube t5 = 
     let h0 = ST.get() in
     let h0 = ST.get() in 
-  Hacl.Impl.EC.PointAdd.computex3_point_add #c hCube uh r t5; 
-  Hacl.Impl.EC.PointAdd.computeY3_point_add #c s1 hCube uh r t5;
+  computex3_point_add #c hCube uh r t5; 
+  computeY3_point_add #c s1 hCube uh r t5;
     let h1 = ST.get() in 
     lemma_coord_eval c h0 h1 p;
     lemma_coord_eval c h0 h1 q;
-  computeZ3_point_add_mixed #c p q h t5;
+  computeZ3_point_add #c p q h t5;
     let h2 = ST.get() in
     lemma_coord_eval c h1 h2 p;
     lemma_coord_eval c h1 h2 q; 
-  copy_point_conditional_affine_to_result result q p t5; 
-  copy_point_conditional result p q
+  copy_result_point_add t5 p q result;
+    let h3 = ST.get() in
+    lemma_coord_eval c h0 h1 p;
+    lemma_coord_eval c h0 h1 q;
+    lemma_point_add_if #c p q result t5 u1 u2 s1 s2 r h uh hCube h0 h2 h3
 
 
 inline_for_extraction noextract
@@ -415,7 +597,6 @@ val _point_add_if_second_branch_impl: #c: curve -> result: point c
       z3 == toDomain #c (pzD * qzD * hD % prime))))
 
 
-
 let _point_add_if_second_branch_impl #c result p q x3hCube t5 = 
   [@inline_let]
   let len = getCoordinateLenU64 c in 
@@ -450,31 +631,29 @@ val _point_add0: #c: curve -> p: point c -> q: point c -> t12: lbuffer uint64 (s
     s1Invariant #c h0 h1 s1 p q /\ s2Invariant #c h0 h1 s2 p q /\ 
     hInvariant #c h1 h u1 u2 /\ rInvariant #c h1 r s1 s2 /\
     uhInvariant #c h1 uh h u1 /\ hCubeInvariant #c h1 hCube h))
- 
+      
 let _point_add0 #c p q t12 = 
   [@inline_let]
   let len = getCoordinateLenU64 c in 
   let h0 = ST.get() in 
   
-  move_from_jacobian_coordinates_mixed p q t12;
-  Hacl.Impl.EC.PointAdd.compute_common_params_point_add t12;
+  move_from_jacobian_coordinates p q t12;
+  compute_common_params_point_add t12;
   let h1 = ST.get() in
   lemma_point_eval c h0 h1 p;
   lemma_point_eval c h0 h1 q 
 
 
 inline_for_extraction noextract
-val point_add_mixed_ : #c: curve -> p: point c -> q: pointAffine c -> result: point c 
+val point_add_mixed_: #c: curve -> p: point c -> q: point c -> result: point c 
   -> tempBuffer: lbuffer uint64 (size 17 *! getCoordinateLenU64 c) -> 
   Stack unit (requires fun h -> 
     live h p /\ live h q /\ live h result /\ live h tempBuffer /\ 
     eq_or_disjoint q result /\ disjoint p q /\ disjoint p tempBuffer /\ 
     disjoint q tempBuffer /\ disjoint p result /\ disjoint result tempBuffer /\  
-    point_eval c h p /\ 
-      (let x, y = getXAff q, getYAff q in 
-      felem_eval c h x /\ felem_eval c h y))
+    point_eval c h p /\ point_eval c h q)
   (ensures fun h0 _ h1 -> modifies (loc tempBuffer |+| loc result) h0 h1 /\ point_eval c h1 result /\
-    fromDomainPoint #c #DH (point_as_nat c h1 result) == _point_add_mixed #c (fromDomainPoint #c #DH (point_as_nat c h0 p)) (fromDomainPointAffine #c (point_affine_as_nat c h0 q)))
+    fromDomainPoint #c #DH (point_as_nat c h1 result) == _point_add #c (fromDomainPoint #c #DH (point_as_nat c h0 p)) (fromDomainPoint #c #DH (point_as_nat c h0 q)))
 
 
 let point_add_mixed_ #c p q result tempBuffer = 
@@ -558,7 +737,6 @@ let point_add_mixed_ #c p q result tempBuffer =
     (==) {_ by (canon())}
     (hD * pzD * qzD) % prime;
   }
-
 
 
 let point_add_mixed_p256 = point_add_mixed_ #P256
