code/ecdsa/Hacl.Impl.EC.Core.fst
@@ -575,7 +575,9 @@ val secretToPublic_0: #c: curve -> #t: buftype -> q: point c -> result: point c 
 
 let secretToPublic_0 #c q result scalar tempBuffer = 
   uploadStartPointsS2P q result; 
-  montgomery_ladder q result scalar tempBuffer
+(*   montgomery_ladder q result scalar tempBuffer *)
+  Hacl.Impl.EC.Masking.ScalarAccess.montgomery_ladder_2_precomputed result scalar tempBuffer;
+  copy q result
 
 
 let secretToPublic #c result scalar tempBuffer = 
